@prefix :        <http://vocab.acousti.ca/bioacoustica#> .
@prefix owl:     <http://www.w3.org/2002/07/owl#> .
@prefix rdf:     <http://www.w3.org/1999/02/22-rdf-syntax-ns#> .
@prefix terms:   <http://purl.org/dc/terms/> .
@prefix oboInOwl:  <http://www.geneontology.org/formats/oboInOwl#> .
@prefix xsd:     <http://www.w3.org/2001/XMLSchema#> .
@prefix rdfs:    <http://www.w3.org/2000/01/rdf-schema#> .
@prefix attributes:  <http://rs.tdwg.org/dwc/terms/attributes/> .
@prefix terms1:  <http://rs.tdwg.org/dwc/terms/> .
@prefix obo:     <http://purl.obolibrary.org/obo/> .

:IsolatedSyllableRepetitionTime
      a       owl:Class ;
      rdfs:subClassOf :SongStructure .

:SyllableDuration_InEcheme
      a       owl:Class ;
      rdfs:subClassOf :SongStructure .

:SyllableDuration_IsolatedSyllable
      a       owl:Class ;
      rdfs:subClassOf :SongStructure .

:hasPropagationMedium
      a       owl:ObjectProperty ;
      rdfs:domain
              [ a       owl:Restriction ;
                owl:onProperty :hasPropagationMedium ;
                owl:someValuesFrom :Call
              ] ;
      rdfs:subPropertyOf owl:topObjectProperty .

:CommunicationDistance
      a       owl:Class ;
      rdfs:comment "e.g. \"near-field\"" .

:EchemeSequenceSpacing
      a       owl:Class ;
      rdfs:subClassOf :SongStructure .

:HearingMechanism
      a       owl:Class .

:SoundPropagationMedium
      a       owl:Class ;
      rdfs:comment "The medium through which the sound is propagated (e.g. air, water, soil). Usually this can be a term from the Environment Ontology."@en .

:EchemeDuration
      a       owl:Class ;
      rdfs:subClassOf :SongStructure .

:EchemesPerEchemeSequence
      a       owl:Class ;
      rdfs:subClassOf :SongStructure .

:HearingPeakSensitivity
      a       owl:Class ;
      rdfs:subClassOf :HearingMechanism .

terms:description
      a       owl:AnnotationProperty .

terms:issued
      a       owl:AnnotationProperty .

:SoundProductionMethod
      a       owl:Class ;
      rdfs:comment "How the organism produces sound. The BioAcoustica SoundProduction ontology (http://vocab.acousti.ca/soundproduction) provides many common use cases."@en .

:SyllablePeriod
      a       owl:Class ;
      rdfs:subClassOf :SongStructure .

:AgressionCall
      a       owl:Class ;
      rdfs:subClassOf :Call .

:TimeOfDay
      a       owl:Class ;
      rdfs:comment "What time of day is the call made?" .

obo:IAO_0000115
      a       owl:AnnotationProperty .

terms:title
      a       owl:AnnotationProperty .

:SyllableSpacing
      a       owl:Class ;
      rdfs:subClassOf :SongStructure .

:EchemePeriod
      a       owl:Class ;
      rdfs:subClassOf :SongStructure .

:SyllableToothImpacts
      a       owl:Class ;
      rdfs:subClassOf :SongStructure .

terms:replaces
      a       owl:AnnotationProperty .

terms:bibliographicCitation
      a       owl:AnnotationProperty .

terms:date
      a       owl:AnnotationProperty .

:TimeOfHighestAcousticActivity
      a       owl:Class ;
      rdfs:comment """e.g. 
0900-1800
Sunrise-1200
Sunrise-sunset
Sunrise-0900; 1800-sunset""" ;
      rdfs:subClassOf :TimeOfDay .

:SyllablesPerEcheme
      a       owl:Class ;
      rdfs:subClassOf :SongStructure .

terms:publisher
      a       owl:AnnotationProperty .

:AlarmCall
      a       owl:Class ;
      rdfs:subClassOf :Call .

:EchemeSequenceDuration
      a       owl:Class ;
      rdfs:subClassOf :SongStructure .

:MaleFemaleDuet
      a       owl:Class ;
      rdfs:subClassOf :Call .

:EchemeSpacing
      a       owl:Class ;
      rdfs:subClassOf :SongStructure .

:FrequencySpectrum
      a       owl:Class ;
      rdfs:comment "in KHz" .

terms:identifier
      a       owl:AnnotationProperty .

:EchemeSequencePeriod
      a       owl:Class ;
      rdfs:subClassOf :SongStructure .

:PeakFrequency
      a       owl:Class ;
      rdfs:subClassOf :FrequencySpectrum .

:FrequencySpectrumPeakEnergy
      a       owl:Class ;
      rdfs:subClassOf :FrequencySpectrum .

:TerritorialCall
      a       owl:Class ;
      rdfs:subClassOf :Call .

:hasCallType
      a       owl:ObjectProperty ;
      rdfs:range
              [ a       owl:Restriction ;
                owl:onProperty :hasCallType ;
                owl:someValuesFrom :Call
              ] ;
      rdfs:subPropertyOf owl:topObjectProperty .

:AdvertismentCall
      a       owl:Class ;
      rdfs:subClassOf :Call .

:hasProductionMethod
      a       owl:TransitiveProperty , owl:ObjectProperty ;
      rdfs:domain
              [ a       owl:Restriction ;
                owl:onProperty :hasProductionMethod ;
                owl:someValuesFrom :Call
              ] ;
      rdfs:range
              [ a       owl:Restriction ;
                owl:onProperty :hasProductionMethod ;
                owl:someValuesFrom :SoundProductionMethod
              ] ;
      rdfs:subPropertyOf owl:topObjectProperty .

terms:modified
      a       owl:AnnotationProperty .

:SyllableDuration_ClosingSyllable
      a       owl:Class ;
      rdfs:subClassOf :SyllableDuration_InEcheme .

<http://vocab.acousti.ca/bioacoustica>
      a       owl:Ontology ;
      rdfs:comment """Ontology to describe the bioacoustic behaviours of animals.

For practical reasons vibrational communication via a substrate is included."""@en ;
      terms:title "BioAcoustica Ontology"@en .

:HearingRange
      a       owl:Class .

:SongStructure
      a       owl:Class .

terms:hasVersion
      a       owl:AnnotationProperty .

:hasCallParticipants
      a       owl:ObjectProperty ;
      rdfs:domain
              [ a       owl:Restriction ;
                owl:onProperty :hasCallParticipants ;
                owl:someValuesFrom :Call
              ] ;
      rdfs:subPropertyOf owl:topObjectProperty .

:Call
      a       owl:Class .
